Changes in Statistics and test case addition

Source/DafnyStandardLibraries/src/Std/Statistics.dfy
@@ -1,8 +1,91 @@
-
+module ExternalMath {
+  function {:extern} Sqrt(x: real): real
+    requires x >= 0.0
+    ensures Sqrt(x) >= 0.0
+    ensures var result := Sqrt(x); result * result <= x + 0.0000001
+    ensures var result := Sqrt(x); result * result >= x - 0.0000001
+}
 
 module Std.Statistics {
-  
+  import opened ExternalMath
   import opened Std.Collections.Seq
+
+  // A function to sum the elements of a sequence
+  function Sum(s: seq<real>): real
+  {
+    if |s| == 0 then
+      0.0
+    else
+      s[0] + Sum(s[1..])
+  }
+
+  // A function to compute the mean (average) as a real number
+  function Mean(s: seq<real>): real
+    requires |s| > 0
+    ensures Mean(s) == Sum(s) / (|s| as real)
+  {
+    Sum(s) / (|s| as real)
+  }
+
+  // A helper function to calculate the sum of squared differences from a given mean
+  function SumSquaredDifferences(s: seq<real>, avg: real): real
+    ensures SumSquaredDifferences(s, avg) >= 0.0
+  {
+    if |s| == 0 then
+      0.0
+    else
+      var diff := s[0] - avg;
+      diff * diff + SumSquaredDifferences(s[1..], avg)
+  }
+  // Function to calculate the absolute value of a real number
+  function RealAbs(x: real): real
+    ensures RealAbs(x) >= 0.0
+    ensures RealAbs(x) == x || RealAbs(x) == -x
+  {
+    if x >= 0.0 then x else -x
+  }
+  // Function to check if two real numbers are close within a given tolerance.
+  function AreNear(a: real, b: real, epsilon: real): bool
+    requires epsilon >= 0.0
+    ensures AreNear(a, b, epsilon) == (RealAbs(a - b) <= epsilon)
+  {
+    RealAbs(a - b) <= epsilon
+  }
+
+  // A function to calculate Population Variance
+  function VariancePopulation(s: seq<real>): real
+    requires |s| > 0
+    ensures VariancePopulation(s) >= 0.0
+    ensures VariancePopulation(s) == SumSquaredDifferences(s, Mean(s)) / (|s| as real)
+  {
+    var avg := Mean(s);
+    SumSquaredDifferences(s, avg) / (|s| as real)
+  }
+
+  // A function to calculate Sample Variance
+  function VarianceSample(s: seq<real>): real
+    requires |s| > 1
+    ensures VarianceSample(s) >= 0.0
+  {
+    var avg := Mean(s);
+    (SumSquaredDifferences(s, avg)) / ((|s| - 1) as real)
+  }
+
+  // A function to calculate Population Standard Deviation
+  function StdDevPopulation(s: seq<real>): real
+    requires |s| > 0
+    ensures StdDevPopulation(s) >= 0.0
+  {
+    ExternalMath.Sqrt(VariancePopulation(s))
+  }
+
+  // A function to calculate Sample Standard Deviation
+  function StdDevSample(s: seq<real>): real
+    requires |s| > 1
+    ensures StdDevSample(s) >= 0.0
+  {
+    ExternalMath.Sqrt(VarianceSample(s))
+  }
 
   // Median of a non-empty sequence of real numbers
   function Median(a: seq<real>): real
